\section{Joint Density Derivation }

\subsection{Proof of Lemma~\ref{lem: joint density}}\label{subsec: joint density derivation}

In this section we want to derive the joint density of \((\nabla^2\rf,\rf):=
(\nabla^2\rf(0), \rf(0))\). As \(\partial_{ij}\rf\) are limits of differences
of multivariate normal random variables, this is a centered multivariate normal
random vector. We therefore only need to consider the covariance. Additionally
we know \(\partial_{ij}\rf = \partial_{ji}\rf\), so we are only interested
in \(((\partial_{ij}\rf)_{i\le j}, \rf)\).

As for the covariances, we have \fxnote{reference}
\begin{align*}
	\Cov(\phi,\phi) &= \dimension \sqC(0)\\
	\Cov(\partial_{ij}\phi,\phi) &= \delta_{ij} \sqC'(0)\\
	\Cov(\partial_{ij}\phi, \partial_{kl}\phi) &= \frac{\sqC''(0)}\dimension
	[\delta_{ij}\delta_{kl} + \delta_{ik}\delta_{jl} + \delta_{il}\delta_{kj}].
\end{align*}
In particular for \(i<j\), we have
\[
	\Cov(\partial_{ij}\phi, \phi) = 0,
\]
and also
\[
	\Cov(\partial_{ij}\phi, \partial_{kl}\phi) = \frac{\sqC''(0)}\dimension
	[\delta_{ik}\delta_{jl} + \underbrace{\delta_{il}\delta_{kj}}_{=0}],
\]
because \(\delta_{il}\delta_{kj}=1\) would imply \(i < j = k \le l = i\), which
is a contradiction. So this covariance is only non-zero, if \(i=k\) and \(j=l\),
i.e. \(\partial_{ij}\phi\) for \(i<j\) has covariance zero with all other terms.
As we are in the multivariate Gaussian case, this also implies independence.
Shifting all these independent mixed derivatives to the end, our covariance
matrix looks like
\[
	\Sigma := \Cov((\partial_{ii}\phi)_{i\le\dimension}, \phi, (\partial_{ij}\phi)_{i<j})
	= \begin{pmatrix}
		B & 0\\
		0 & \frac{\sqC''(0)}{\dimension}\identity
	\end{pmatrix}
\]
with
\[
	B = \begin{pmatrix}
		3\frac{\sqC''(0)}\dimension &  \cdots & \frac{\sqC''(0)}\dimension
		& \sqC'(0) \\
		\vdots & \ddots &\vdots & \vdots \\
		\frac{\sqC''(0)}\dimension & \cdots &  3 \frac{\sqC''(0)}\dimension & \sqC'(0)\\
		\sqC'(0)	& \cdots & \sqC'(0) & \dimension \sqC(0)
	\end{pmatrix}
	=: \begin{pmatrix}
		\Sigma_\partial & b \\
		b^T & d
	\end{pmatrix}.
\]
Inverting \(\Sigma\) is easy, if we can invert \(B\). If we can invert the
covariance of partial derivatives \(\Sigma_\partial\), we have
\[
	B^{-1} = \frac1{d- b^T \Sigma_\partial^{-1}b}\begin{pmatrix}
		( d- b^T \Sigma_\partial^{-1}b )\Sigma_\partial^{-1}
		+ \Sigma_\partial^{-1}b b^T \Sigma_\partial^{-1}
		& -\Sigma_\partial^{-1} b\\
		-b^T\Sigma_\partial ^{-1} &  1
	\end{pmatrix},
\]
as one can verify by calculating \(BB^{-1}\). As \(\Sigma_\partial\) is of the form
\[
	\Sigma_\partial=\frac{\sqC''(0)}{\dimension}[2\identity + \ones\ones^T]
\]
with \(\ones=(1,\dots,1)^T\in\real^\dimension\), we can use the Sherman-Morrison
formula.

\begin{lemma}[Sherman-Morrison Formula]
	Let \(A\) be an invertible matrix, \(u,v\in\real^\dimension\) column vectors.
	Then \(A+ uv^T\) is invertible iff \(1+v^T A^{-1}u \neq 0\), and if that is
	the case, we have
	\[
		(A+uv^T)^{-1} = A^{-1} - \frac{A^{-1}u v^T A^{-1}}{1+v^T A^{-1}u}.
	\]
\end{lemma}
\begin{proof}
	Multiply \((A+uv^T)\) with its proposed inverse.
\end{proof}

The application of this formula results in
\begin{equation}\label{eq: sigma_partial inverse}
	\Sigma_\partial^{-1}
	= \frac{\dimension}{\sqC''(0)}\left[
		\tfrac12\identity - \frac{\tfrac14\ones\ones^T}{1+\tfrac12\ones^T\ones}
	\right]
	= \frac{\dimension}{2\sqC''(0)}\left[
		\identity - \frac{1}{2+\dimension}\ones\ones^T
	\right].
\end{equation}
To determine \(B^{-1}\), we first define
\begin{align*}
	q := d - b^T \Sigma_\partial^{-1}b
	&= \dimension\sqC(0) - \tfrac{\dimension\sqC'(0)^2}{2\sqC''(0)}\ones^T
	[\identity-\tfrac1{2+\dimension}\ones\ones^T]\ones\\
	&= \dimension\left[
		\sqC(0) - \tfrac{\sqC'(0)^2}{2\sqC''(0)}
		\dimension( 1-\tfrac{\dimension}{2+\dimension} )
	\right]\\
	&= \dimension\left[
		\sqC(0) - \tfrac{\sqC'(0)^2}{\sqC''(0)}
		\tfrac{\dimension}{2+\dimension}
	\right],
\end{align*}
and then calculate
\begin{equation}\label{eq: definition of c=sigma_partial^{-1} b}
	c:=\Sigma_\partial^{-1}b
	= \tfrac{\dimension\sqC'(0)}{2\sqC''(0)}( 1 - \tfrac{\dimension}{2+\dimension} )\ones
	= \tfrac{\sqC'(0)}{\sqC''(0)}\tfrac{\dimension}{2+\dimension}\ones.
\end{equation}
Therefore we have
\begin{equation}\label{eq: inv B split}
	B^{-1} = \begin{pmatrix}
		\Sigma_\partial^{-1}	+ \frac{cc^T}{q} & - \frac{c}{q}\\
		-\frac{c^T}{q} & \frac1q
	\end{pmatrix}
	= \begin{pmatrix}
		\Sigma_\partial^{-1} & 0 \\
		0 & 0
	\end{pmatrix}
	+ \frac1q \begin{pmatrix}
		cc^T & -c\\
		-c^T & 1
	\end{pmatrix}.
\end{equation}

Let us take a step back now. We want to calculate
\begin{equation*}
	p(H, \phi)
	=C_\dimension\exp\left(
		-\tfrac12
		( H_{ii},\phi, H_{ij} )\Sigma^{-1}
		\begin{pmatrix}
			H_{ii}\\
			\phi\\
			H_{ij}
		\end{pmatrix}
	\right)
\end{equation*}
where we abbreviate for readability \((H_{ii}, \phi, H_{ij})= ((H_{ii})_{i\le
\dimension}, \phi, (H_{ij})_{i<j})\) and define
\begin{align*}
	C_\dimension &:= \left((2\pi)^{n(\dimension)}\det(\Sigma)\right)^{-1/2}\\
	n(\dimension) &:= 1 + \tfrac{\dimension(\dimension+1)}{2}.
\end{align*}
Looking at just the exponent we have
\begin{align*}
		\tfrac12
		( H_{ii},\phi, H_{ij} )\Sigma^{-1}
		\begin{pmatrix}
			H_{ii}\\
			\phi\\
			H_{ij}
		\end{pmatrix}
		&= 
		\tfrac12
		( H_{ii},\phi, H_{ij} )\begin{pmatrix}
			B^{-1} & 0\\
			0 & \tfrac{\dimension}{\sqC''(0)}\identity
		\end{pmatrix}
		\begin{pmatrix}
			H_{ii}\\
			\phi\\
			H_{ij}
		\end{pmatrix}\\
		&= \tfrac12(H_{ii},\phi)B^{-1}\begin{pmatrix}
			H_{ii}\\ \phi
		\end{pmatrix}
		+ \underbrace{\tfrac{\dimension}{2\sqC''(0)}\| (H_{ij})_{i<j}\|^2}_{
			=\tfrac{\dimension}{4\sqC''(0)}\| (H_{ij})_{i\neq j}\|^2.
		}
\end{align*}
For the first part we can use \eqref{eq: inv B split} to get
\[
		\tfrac12(H_{ii},\phi)B^{-1}\begin{pmatrix}
			H_{ii}\\ \phi
		\end{pmatrix}
		= \frac12 
			H_{ii} \Sigma_\partial^{-1} H_{ii}
			+
			\underbrace{
				\frac1{2q}
				(H_{ii},\phi)
				\begin{pmatrix}
					cc^T & -c \\
					-c^T & 1
				\end{pmatrix}
				\begin{pmatrix}
					H_{ii}\\ \phi
				\end{pmatrix}
			}_{=: \dimension S_1(H, \phi)}.
\]
Using \eqref{eq: sigma_partial inverse}, we also obtain
\[
	\frac12 H_{ii} \Sigma_\partial^{-1} H_{ii}
	= \frac{\dimension}{4\sqC''(0)}
	\left[\|H_{ii}\|^2 - \tfrac{(\trace H)^2}{2+\dimension}\right].
\]
Putting the last three equations back together, we get
\begin{align*}
		\tfrac12
		( H_{ii},\phi, H_{ij} )\Sigma^{-1}
		\begin{pmatrix}
			H_{ii}\\
			\phi\\
			H_{ij}
		\end{pmatrix}
		&= \underbrace{
			\tfrac{\dimension}{4\sqC''(0)}\left[
			\|(H_{ij})_{ij}\|^2
			- \tfrac{(\trace H)^2}{2+\dimension}
		\right]
		}_{=: \dimension^2 S_2(H)}
		+ \dimension S_1(H,\phi),
\end{align*}
where we joined the norm over the diagonal elements with the norm over the rest.
This can be further simplified to
\begin{align*}
	\|(H_{ij})_{ij}\|^2 = \sum_{i,j=1}^\dimension H_{ij}^2
	= \sum_{i=1}^\dimension \underbrace{\sum_{j=1}^\dimension H_{ij}H_{ji}}_{(H^2)_{ii}}
	= \trace(H^2).
\end{align*}
As claimed in Lemma~\ref{lem: joint density}, we therefore have
\[
	S_2(H) = \frac{1}{4 \dimension \sqC''(0)} \left[
		\trace H^2 - \frac{(\trace H)^2}{2+\dimension}
	\right].
\]
Now we just need to prove that the \(S_1\) we defined here, is also the same as
in the Lemma. For that recall the definition of \(c\) in \eqref{eq: definition of
c=sigma_partial^{-1} b} and the definition of \(q\) which resulted in
\[
	c=\tfrac{\sqC'(0)}{\sqC''(0)}\tfrac{\dimension}{2+\dimension}\ones
	\qquad \text{and} \qquad
	q=\dimension\left[
		\sqC(0) - \tfrac{\sqC'(0)^2}{\sqC''(0)}
		\tfrac{\dimension}{2+\dimension}
	\right].
\]
As a first result, we get
\[
	\langle c, H_{ii}\rangle = 
	\tfrac{\sqC'(0)}{\sqC''(0)}\tfrac{\dimension}{2+\dimension}\trace H.
\]
Now we apply this to \(S_1\), resulting in
\begin{align*}
	S_1(H, \phi)
	&= \frac{1}{2\dimension q}
	(H_{ii},\phi)
	\begin{pmatrix}
		cc^T & -c \\
		-c^T & 1
	\end{pmatrix}
	\begin{pmatrix}
		H_{ii}\\ \phi
	\end{pmatrix}\\
	&= \frac1{2\dimension q}
	\left[\langle c, H_{ii}\rangle^2 - 2\langle c, H_{ii}\rangle + \phi^2\right]
	\\
	&= \frac1{2\dimension q}
	\left[
		\left(\tfrac{\sqC'(0)}{\sqC''(0)}\tfrac{\dimension}{2+\dimension}\right)^2(\trace H)^2
		- 2\tfrac{\sqC'(0)}{\sqC''(0)}\tfrac{\dimension}{2+\dimension} \phi\trace H
		+ \phi^2
	\right].
\end{align*}
Finally note, that
\[
	q = \frac{\dimension^2\sqC''(0)}{\dimension+2}
	\underbrace{
	\left[
		\frac{\dimension +2}{\dimension}\frac{\sqC(0)}{\sqC''(0)} - \frac{\sqC'(0)^2}{\sqC''(0)^2}
	\right]
	}_{=:Q},
\]
as this concludes our proof of Lemma~\ref{lem: joint density}:
\begin{align*}
	S_1(H, \phi)
	&= \frac1{2\dimension Q}\frac{\dimension+2}{\dimension^2\sqC''(0)}
	\left[
		\left(\tfrac{\sqC'(0)}{\sqC''(0)}\tfrac{\dimension}{2+\dimension}\right)^2(\trace H)^2
		- 2\tfrac{\sqC'(0)}{\sqC''(0)}\tfrac{\dimension}{2+\dimension}\phi \trace H
		+ \phi^2
	\right]\\
	&= \frac1{2\sqC''(0)Q}\frac{\dimension+2}{\dimension^3}
	\left[
		\left(\tfrac{\sqC'(0)}{\sqC''(0)}\tfrac{\dimension}{2+\dimension}\right)^2(\trace H)^2
		- 2\tfrac{\sqC'(0)}{\sqC''(0)}\tfrac{\dimension}{2+\dimension} \phi\trace H
		+ \phi^2
	\right]\\
	&= \frac1{2\sqC''(0)Q}
	\left[
		\tfrac{\sqC'(0)^2}{\sqC''(0)^2\dimension(2+\dimension)}(\trace H)^2
		- 2\tfrac{\sqC'(0)}{\dimension^2\sqC''(0)}\phi\trace H
		+ \tfrac{\dimension+2}{\dimension^3}\phi^2
	\right].
\end{align*}